Bellman.dfy
@@ -40,7 +40,7 @@ predicate isValid(graph: Graph)
 }
 
 
-method Main(){
+method dada(){
   var node1 := V(1);
   var node2 := V(2);
   var node3 := V(3);
@@ -95,7 +95,7 @@ function MyIntLessThan(x: MyInt, y: MyInt): bool
     case MinValue => false
     case Valid(n) =>
       match y {
-        case MinValue => false
+        case MinValue => true
         case Valid(m) => n < m
       }
   }
@@ -109,41 +109,40 @@ ghost predicate Length_Ver(edges: seq<New_Edge>, distanceLength: nat)
   forall edge :: edge in edges ==>
                    0 <= edge.source.id < distanceLength && 0 <= edge.destination.id < distanceLength
 }
-
 method Relax_Edges(source: Node, predecessor: array<int>, edges: array<New_Edge>, distance: array<MyInt>)
   modifies distance, predecessor
   requires distance.Length > 0 && edges.Length > 0 && predecessor.Length > 0
   requires predecessor.Length == distance.Length
 {
-  var i: nat := 0;
-
-  while i < distance.Length - 1
-    invariant 0 <= i <= distance.Length - 1
+  var k: nat := 0;
+  while k < distance.Length - 1
   {
     var j: nat := 0;
-
     while j < edges.Length
-      invariant 0 <= j <= edges.Length
     {
       var edge := edges[j];
       var u := edge.source.id;
       var v := edge.destination.id;
       var w := edge.weight.val;
 
-      if 0 <= u < distance.Length && 0 <= v < distance.Length && 0 <= v < predecessor.Length
+      if 0 <= u < distance.Length && 0 <= v < distance.Length
       {
-        if distance[u] != MinValue && MyIntLessThan(MyIntAdd(distance[u], w), distance[v])
+        if distance[u] != MinValue
         {
-          distance[v] := MyIntAdd(distance[u], w);
-          predecessor[v] := u;
+          var newDist := MyIntAdd(distance[u], w);
+          if newDist != MinValue && (distance[v] == MinValue || MyIntLessThan(newDist, distance[v]))
+          {
+            distance[v] := newDist;
+            predecessor[v] := u;
+          }
         }
       }
       j := j + 1;
     }
-    i := i + 1;
+    k := k + 1;
   }
-
 }
+
 
 method Detect_Negative_Cycle(edges: array<New_Edge>, distance: array <MyInt>)
   returns (hasNegativeCycle: bool)
@@ -195,11 +194,53 @@ method BellmanFord(source: Node, predecessor: array<int>, edges: array<New_Edge>
     i := i + 1;
   }
 
-  if 0 <= source.id < distance.Length {
-    distance[source.id] := Valid(0);
-  }
+  distance[source.id] := Valid(0);
+
 
   Relax_Edges(source, predecessor, edges, distance);
 
   hasNegativeCycle := Detect_Negative_Cycle(edges, distance);
+}
+
+method Main()
+{
+  var node0 := V(0);
+  var node1 := V(1);
+  var node2 := V(2);
+  var node3 := V(3);
+
+  var edges := new New_Edge[5];
+  edges[0] := Edge_new(node0, node1, W_new(Valid(4)));  // 0 -> 1 cu cost 4
+  edges[1] := Edge_new(node0, node2, W_new(Valid(2)));  // 0 -> 2 cu cost 2
+  edges[2] := Edge_new(node1, node2, W_new(Valid(-3))); // 1 -> 2 cu cost -3
+  edges[3] := Edge_new(node2, node3, W_new(Valid(2)));  // 2 -> 3 cu cost 2
+  edges[4] := Edge_new(node1, node3, W_new(Valid(3)));  // 1 -> 3 cu cost 3
+
+  var distance := new MyInt[4];
+  var predecessor := new int[4];
+
+  var hasNegativeCycle := BellmanFord(node0, predecessor, edges, distance);
+
+  print "Neg cicl ", hasNegativeCycle, "\n";
+  print "Dist de la nodul sursa (0):\n";
+
+  var i := 0;
+  while i < distance.Length
+  {
+    print "La nodul ", i, ": ";
+    match distance[i] {
+      case MinValue => print "Infinit";
+      case Valid(n) => print n;
+    }
+    print "\n";
+    i := i + 1;
+  }
+
+  print "Pred:\n";
+  i := 0;
+  while i < predecessor.Length
+  {
+    print "Pentru nodul ", i, ": ", predecessor[i], "\n";
+    i := i + 1;
+  }
 }
